\begin{frame}[fragile]
	\frametitle{Canonical Example}
	\begin{lstlisting}
 while ( F = 0 ) {
   { X := X - 1 }[0.5]{ F := 1 }
 }
	\end{lstlisting}
	\begin{itemize}
		\itemspacing{10pt}
		\item<2-> $ \smtx{\while{B}{P}}(G) = 
			\sum\limits_{i = 0}^{\infty} \alert<3>{ \resN{\wh^i(G)} } $
		\item<4-> $ B = (F = 0) $
		\item<5-> $ P = \{ X := X - 1 \}[0.5]\{ F := 1 \} $
		\item<6-> $ G = 1 X^0 F^0 = 1 $
	\end{itemize}
\end{frame}

\begin{frame}
	\frametitle{Canonical Example}
	\begin{itemize}[<+->]
		\itemspacing{10pt}
		\item $ \resN{\wh^1(1)} = \hf X^0 F^1 $
		\item $ \resN{\wh^2(1)} = \qu X^{-1} F^1 $
%		\item $ \ldots $
		\item $\resN{\wh^n(1)} = \half^n X^{-(n-1)} F^1 $
		\item $ \sum\limits_{i = 0}^{\infty} \resN{\wh^i(G)}
			= \alert<.>{\hf \cdot \sum\limits_{i = 0}^{\infty} \half^i X^{-i} F^1} $
		\item Closed form: $ \frac{F}{2 - X^{-1}} $
		\item Actually: $ \pair{0, \frac{F}{2 - X^{-1}}, 0, 0} $
	\end{itemize}
\end{frame}

\begin{frame}[fragile]
\frametitle{Termination Probability}
\begin{lstlisting}
while ( F = 0 ) {
  {
    { X := X + 1 }[0.5]{ diverge }
  }[0.5]{
    F := 1
  }
}
\end{lstlisting}
\begin{itemize}[<+(1)->]
	\itemspacing{10pt}
	\item $ \resN{\wh^i \l(G\r)} = \hf \cdot \l(\frac{1}{4}\r)^{i-1} X^{i-1} F^1 $
	\item $ \sum\limits_{i = 0}^{\infty} \resN{\wh^i(G)}
	= \alert{\hf \cdot \sum\limits_{i = 0}^{\infty} \l(\frac{1}{4}\r)^i X^i F^1} $
\end{itemize}
\end{frame}

\begin{frame}
	\frametitle{Termination Probability}
	\begin{itemize}[<+->]
		\itemspacing{10pt}
		
		\item Closed form: $ \frac{F}{2 - \hf X} $
		\item Termination probability using absolute value:
		\item $ \l| \hf \cdot \sum\limits_{i = 0}^{\infty} \l(\frac{1}{4}\r)^i X^i F^1 \r|
			\uncover<+->{
				= \hf \cdot \sum\limits_{i = 0}^{\infty} \l(\frac{1}{4}\r)^i 
			}
			\uncover<+->{
				=  \frac{2}{3}
			} $
		\item $ \l| \frac{F}{2 - \hf X} \r| = \frac{1}{2 - \hf} = \frac{2}{3} $
	\end{itemize}
\end{frame}

\begin{frame}[fragile]
	\frametitle{Equivalent Programs}
	\begin{columns}
		\begin{column}[t]{0.5\textwidth}
			\begin{lstlisting}[basicstyle=\scriptsize]
while ( F = 0 ) {
  { X := X + 1 }[p]{ F := 1 }
};
 
F := 0;
while ( F = 0 ) {
  { X := X - 1 }[q]{ F := 1 }
}
			\end{lstlisting}
		\end{column}
		\hspace{-20pt}
		{ \vrule width 1pt }
%		\vrule{}
		\hspace{7pt}
		\begin{column}[t]{0.5\textwidth}
			\begin{lstlisting}[basicstyle=\scriptsize]
{ F := 0 }[0.5]{ F := 1 };
if ( F = 0 ) {
  while ( F = 0 ) {
    { X := X + 1 }[p]{ F := 1 }
  }

} else {
  F := 0;
  while ( F = 0 ) {
    X := X - 1;
    { skip }[q]{ F := 1 }
  }
}
			\end{lstlisting}
		\end{column}
	\end{columns}
\end{frame}

\begin{frame}[fragile]
	\frametitle{Equivalent Programs}
	\begin{columns}
		\begin{column}[t]{0.5\textwidth}
			\begin{lstlisting}[basicstyle=\tiny]
while ( F = 0 ) {
  { X := X + 1 }[p]{ F := 1 }
};

F := 0;
while ( F = 0 ) {
  { X := X - 1 }[q]{ F := 1 }
}
			\end{lstlisting}
		\end{column}
		\begin{column}[t]{0.5\textwidth}
			\begin{lstlisting}[basicstyle=\tiny]
{ F := 0 }[0.5]{ F := 1 };
if ( F = 0 ) {
  while ( F = 0 ) {
    { X := X + 1 }[p]{ F := 1 }
  }

} else {
  F := 0;
  while ( F = 0 ) {
    X := X - 1;
    { skip }[q]{ F := 1 }
  }
}
			\end{lstlisting}
		\end{column}
	\end{columns}
	\begin{itemize}[<+->]
		\item Introduced by Kiefer et al. in 2012.
		\item Proven equivalent in distribution for $p = \frac{1}{2}$ and $q = \frac{2}{3}$.
		\item Expected value of $X$ is the same if $q = \frac{1}{2-p}$. (Gretz et al.)
		\item Today: equivalence in distribution if $q = \frac{1}{2-p}$.
	\end{itemize}
\end{frame}

\begin{frame}
	\frametitle{Equivalent Programs}
	\begin{itemize}[<+->]
		\item First program's semantics: \\[10pt]
			$ \alert<.(4)>{ \frac{(1-q) \cdot (1-p)}{1-qp} } \cdot	% factor
			\pair{
				\alert<.(2)>{ \frac{F}{1 - p X} }, \ % first entry sum
				\alert<.(4)>{ q } \cdot	% second entry factor
					\alert<.(3)>{ \frac{X^{-1} F}{1 - q X^{-1}} } % snd entry sum
				, 0, 0 % null entries
			} $
			\vspace*{20pt}
		\item Second program's semantics: \\[10pt]
			$ \pair{
				\alert<.(3)>{ \frac{1-p}{2} } \cdot	% first entry factor
					\alert<.(1)>{ \frac{F}{1 - p X} }, \ % first entry sum
				\alert<.(3)>{ \frac{1-q}{2} } \cdot	% second entry factor
					\alert<.(2)>{ \frac{X^{-1} F}{1 - q X^{-1}} } % snd entry sum
					, 0, 0 % null entries
			} $
			\vspace*{20pt}
		\item<+(3)-> Solve $ \frac{(1-q) \cdot (1-p)}{1-qp} = \frac{1-p}{2} $ and
			$ \frac{(1-q) \cdot (1-p) \cdot q}{1-qp} = \frac{1-q}{2} $.
			\vspace*{10pt}
		\item<+(3)-> Equivalent in distribution if $ q = \frac{1}{2 - p}$.
	\end{itemize}
\end{frame}
