\begin{lemma}[label=lem:bisim:iteration]
	Let $B$ be a boolean condition, $P$ a program and $R$ a basic bisimulation. \\
	Then \[ \pair{K, G} \in R
		\implies \pair{K - \sum_{i = 1}^{n} \resN{\wh^i(G)}, \wh^n(G)}
		\in R \text{ for all } n \in \N \]
	\begin{proof}
		Proof by induction over $n$. \\
		\textbf{Base case} for $n = 0$:
		\begin{align*}
					 & \pair{K, G} \in R \\
			\implies & \pair{K - 0, G} \\
					 & \explain{empty sum} \\
			\implies & \pair{K - \sum_{i = 1}^{0} \resN{\wh(G)}, \wh^0(G)}
		\end{align*}
		\textbf{Induction hypothesis}:
		 \[ \pair{K, G} \in R \implies
			\pair{K - \sum_{i = 1}^{n} \resN{\wh^i(G)}, \wh^{n}(G)} \in R
			\text{ for some } n \in \N \]
		\textbf{Inductive step}: \\
		$R$ is a basic bisimulation, so we can apply the iteration step to the induction hypothesis which yields
		\begin{align*}
				 & \pair{K, G} \in R \\
				 & \explain{induction hypothesis} \\
		\implies & \pair{K - \sum_{i = 1}^{n} \resN{\wh^i(G)}, \wh^{n}(G)} \in R \\
				 & \explain{property ii) of weak bisimulations} \\
		\implies & \pair{K - \sum_{i = 1}^{n} \resN{\wh^i(G)} - \resN{\wh(\wh^n(G))}
			, \wh(\wh^{n}(G))} \in R \\
		\implies & \pair{K - \sum_{i = 1}^{n} \resN{\wh^i(G)} - \resN{\wh^{n+1}(G)}
			, \wh^{n+1}(G)} \in R \\
		\implies & \pair{K - \sum_{i = 1}^{n+1} \resN{\wh^i(G)}
			, \wh^{n+1}(G)} \in R
		\end{align*}
	\end{proof}
\end{lemma}

\begin{theorem}[continues=theo:bisim:overapprox, label=proof:bisim:overapprox]
	Let $B$ be a Boolean condition, $P$ a program and $R$ a weak bisimulation. \\
	Then \[ \pair{K, G} \in R \land G \models B
		\implies \smtx{\while{B}{P}}(G) \leqD K \]
	\begin{proof}
		\begin{align*}
					 & \pair{K, G} \in R \land G \models B \\
					 & \explain{Lemma~\ref{lem:bisim:iteration}} \\
			\implies & \pair{K - \sum_{i = 1}^{n} \resN{\wh^i(G)}, \wh^n(G)} \in R \\
					 & \land \resN{G} = 0 \\
					 & \explain{property i) of weak bisimulations} \\
			\implies & \resN{\wh\left(\wh^n(G)\right)}
				\leqD K - \sum_{i=1}^n \resN{\wh^i(G)} \\
					 & \land \resN{\wh^0(G)} = 0 \\
			\implies & \resN{\wh^0(G)} + \sum_{i=1}^n \resN{\wh^i(G)} + \resN{\wh^{n+1}(G)} \leqD K \\
			\implies & \sum_{i=0}^{n+1} \resN{\wh^i(G)} \leqD K \\
			\implies & \sup_{n \in \N} \sum_{i=0}^{n+1} \resN{\wh^i(G)}
				\leqD \sup_{n \in \N} K \\
			\implies & \smtx{\while{B}{P}}(G) \leqD K
		\end{align*}
	\end{proof}
\end{theorem}

\begin{lemma}[label=lem:bisim:iterateeps]
	Let $B$ be a Boolean condition, $P$ a program and $R$ a strong bisimulation for $B$ and $P$ with constant $\varepsilon$.
	Then,
	\[ \pair{K, G} \in R \implies \l| K \r| - \l| \sum_{i=1}^{n} \resN{\wh^i(G)} \r|
		\leq (1-\varepsilon)^n \cdot |K| \text{ for all } n \in \N \]
	\begin{proof}
		Proof by induction over $n$. \\
		\textbf{Base case} for $n = 0$:
		\[ |K| - \l| \sum_{i=1}^{0} \resN{\wh^i(G)} \r|
			= |K| - |0| \leq 1 \cdot |K| = (1-\varepsilon)^0 \cdot |K| \]
		\textbf{Induction hypothesis}:
		\[ \pair{K, G} \in R \implies \l| K \r| - \l| \sum_{i=1}^{n} \resN{\wh^i(G)} \r|
			\leq (1-\varepsilon)^n \cdot |K| \text{ for some } n \in \N \]
		\textbf{Inductive step}:	%%% REDO
		\begin{align*}
		 & \pair{K, G} \in R \\
		 & \explain{Lemma~\ref{lem:bisim:iteration}} \\
		\implies & \pair{K - \sum_{i=1}^{n+1} \resN{\wh^i(G)}, \wh^n(G)} \in R \\
		 & \explain{Property iii) of strong bisimulations} \\
		\implies & \l| \resN{ \wh\l( \wh^n(G) \r) } \r|
			 \geq \varepsilon \cdot \l| K - \sum_{i=1}^{n} \resN{\wh^i(G)} \r| \\
		 & \explain{negate, add to both sides} \\
		\implies & \l( |K| - \l| \sum_{i=1}^{n} \resN{\wh^i(G)} \r| \r)
			- \l| \resN{ \wh^{n+1}(G) } \r| \\
		 & \leq  \l( |K| - \l| \sum_{i=1}^{n} \resN{\wh^i(G)} \r| \r)
			- \varepsilon \cdot
			\l( |K| - \l| \sum_{i=1}^{n} \resN{\wh^i(G)} \r| \r) \\
		 & \explain{merge sums, factor out} \\
		\implies & |K| - \l| \sum_{i=1}^{n+1} \resN{\wh^i(G)} \r|
			\leq (1-\varepsilon) \cdot 
			\l( |K| - \l| \sum_{i=1}^{n} \resN{\wh^i(G)} \r| \r) \\
		 & \explain{induction hypothesis} \\
		\implies & |K| - \l| \sum_{i=1}^{n+1} \resN{\wh^i(G)} \r|
			\leq (1-\varepsilon) \cdot (1-\varepsilon)^n \cdot |K|
			= (1-\varepsilon)^{n+1} \cdot |K| \\
		\end{align*}
	\end{proof}
\end{lemma}

\begin{lemma}
	\label{lem:leq_and_mass_impl_equality}
	Let $G$ and $G'$ be PGFs of $k$ variables with coefficients $\mu_s$ and $\mu_s'$ for $s \in \Z^k$, respectively. Then
	$$ G \leqD G' \ \land \ |G| = |G'| \implies G = G' $$
	\begin{proof}
		Let $G$ and $G'$ be PGFs as above such that $G \leqD G'$ and $|G| = |G'|$.
		Now assume $G \ne G'$.
		Then there exists $s \in \Z^k$ with $\mu_s \ne \mu_s'$.
		Since $G \leqD G'$ it follows that $\mu_s < \mu_s'$.
		Adding all other coefficients on both sides does not break the inequation as every coefficient of $G$ is less or equal to the respective coefficient of $G'$.
		Hence,
		\[ |G| = \sum_{s \in \Z^k} \mu_s < \sum_{s \in \Z^k} \mu_s' = |G'| \]
		This is a contradiction to the precondition, so $G = G'$.
	\end{proof}
\end{lemma}

\begin{theorem}[continues=theo:bisim:loopsmtx, label=proof:bisim:loopsmtx]
	Let $B$ be a Boolean condition, $P$ a program and $R$ a strong bisimulation for $B$ and $P$ with constant $\varepsilon$. Then
	\[ \pair{K, G} \in R \land G \models B \implies K = \smtx{\while{B}{P}}(G) \]
	\begin{proof}
		\begin{align*}
		 & \pair{K, G} \in R \land G \models B \\
		 & \explain{Lemma \ref{lem:bisim:iterateeps}} \\
		\implies & |K| - \l| \sum_{i=1}^{n} \resN{\wh^i(G)} \r|
			\leq (1-\varepsilon)^n \cdot |K|
			\land \resN{wh^0(G)} = 0 \\
		\implies & |K| - \l| \sum_{i=0}^{n} \resN{\wh^i(G)} \r|
			\leq (1-\varepsilon)^n \cdot |K| \\
		\implies & \lim_{n \to \infty}
		\l( |K| - \l| \sum_{i=0}^{n} \resN{\wh^i(G)} \r| \r)
		\leq \lim_{n \to \infty} (1-\varepsilon)^n \cdot |K| \\
		\implies & \lim_{n \to \infty} \l| K \r| -
		\lim_{n \to \infty} \l| \sum_{i=0}^{n} \resN{\wh^i(G)} \r|
		\leq \lim_{n \to \infty} (1-\varepsilon)^n \cdot |K| \\
		& \text{$a_n = \sum_{i=0}^{n} \resN{\wh^i(G)}$ is monotonic and bounded by its supremum given by the cpo $D$,} \\
		& \text{so $a_n$ converges to its supremum.} \\
		\implies & \lim_{n \to \infty} \l| K \r| -
		\l| \sup_{n \in \N} \sum_{i=0}^{n} \resN{\wh^i(G)} \r|
		\leq \lim\limits_{n \to \infty} (1-\varepsilon)^n \cdot |K| \\
		\implies & \l| K \r| - \l| \smtx{\while{B}{P}}(G) \r| \leq 0 \\
		\implies & \l| K \r| \leq \l| \smtx{\while{B}{P}}(G) \r|
		\end{align*}
		\\
		Using this and Theorem \ref{theo:bisim:overapprox}, we get
		\begin{align*}
		& \pair{K, G} \in R \land G \models B \\
		& \explain{apply Theorem \ref{theo:bisim:overapprox} and the previous result} \\
		\implies & \smtx{\while{B}{P}}(G) \leqD K \land |K| \leq \l| \smtx{\while{B}{P}}(G) \r| \\
		\implies & \l| \smtx{\while{B}{P}}(G) \r| \leq |K| \land
		|K| \leq \l| \smtx{\while{B}{P}}(G) \r| \\
		\implies & |K| = \l| \smtx{\while{B}{P}}(G) \r|
		\end{align*}
		To recap, from $\pair{K, G} \in R \land G \models B$ it follows that
		\begin{itemize}
			\item $\l| \smtx{\while{B}{P}}(G) \r| = |K|$ from above, and
			\item $\smtx{\while{B}{P}}(G) \leqD K$ from Theorem \ref{theo:bisim:overapprox}.
		\end{itemize}
		These satisfy the precondition of Lemma \ref{lem:leq_and_mass_impl_equality},
		which gives us the final result
		\[ \pair{K, G} \in R \land G \models B
			\implies K = \smtx{\while{B}{P}}(G) 		\qedhere \]
	\end{proof}
\end{theorem}