In this proof, we will not show the exact statement for the canonical example, but a more general one.
Therefore, we slightly modify the loop body $P$ by parametrising it with a variable $p\in [0, 1]$.
\[ P_p = \{ X := X + 1 \}[p]\{ F := 1 \} \]
The statement needed for the canonical example then is the special case $p = \hf$.
\begin{lemma}
	Let $B = (F = 0)$ be a Boolean condition and $P_p$ as above with $p \in [0, 1]$.
	Then
	\[ \resN{\operatorname{wh}_{B, P_p}^i\l(1\r)}
		= (1-p) \cdot p^{i-1} X^{i-1} F^1 \where i > 0 \]
	\begin{proof}
		We will prove the equation above without the restriction to $\lnot B$ and apply it afterwards. \\
		Proof by induction over $i$. \\
		\textbf{Base Case} for $i = 1$: \\
		\[ \operatorname{wh}_{B, P_p}^1\l(1\r)
			= p^1 X^1 F^0 + (1-p)^1 X^0 F^1 \]
		\textbf{Induction Hypothesis}:
		\[ \operatorname{wh}_{B, P_p}^i\l(1\r)
			= p^i X^i F^0 + (1-p) \cdot p^{i-1} X^{i-1} F^1 \text{ for some } i > 0 \]
		\textbf{Inductive Step}:
		\begin{align*}
			 & \operatorname{wh}_{B, P_p}^{i + 1}\l(1\r) \\
			=& \operatorname{wh}_{B, P_p}\l(
				\operatorname{wh}_{B, P_p}^i\l(1 \r) \r) \\
			 & \explain{definition of $\operatorname{wh}_{B, P_p}$} \\
			=& \smtx{P}\l( \resP{ \operatorname{wh}_{B, P_p}^i\l(1\r) } \r) \\
			 & \explain{induction hypothesis} \\
			=& \smtx{P}\l( \resP{p^i X^i F^0 + (1-p) \cdot p^{i-1} X^{i-1} F^1} \r) \\
			 & \explain{$B = (F = 0)$} \\
			=& \smtx{P}\l( p^i X^i F^0 \r) \\
			 & \explain{semantics of $P$} \\
			=& p \cdot p^i X^{i+1} F^0 + (1-p) \cdot p^i X^i F^1 \\
			=& p^{i+1} X^{i+1} F^0 + (1-p) \cdot p^i X^i F^1
		\end{align*}
		The intermediate claim is proven by induction.
		The final result is now obtained by restriction to $\lnot B$:
		\[ \resN{\operatorname{wh}_{B, P_p}^i\l(1\r)}
			= \resN{p^i X^i F^0 + (1-p) \cdot p^{i-1} X^{i-1} F^1}
			= (1-p) \cdot p^{i-1} X^{i-1} F^1		\qedhere \]
	\end{proof}
\end{lemma}
Summing all $\wh^i(1)$ gives us the semantics of the more general loop:
\begin{align*}
	 & \smtx{\while{B}{P_p}}(1) \\
	=& \resN{\operatorname{wh}_{B, P_p}^0(1)}
		+ \sum_{i = 1}^{\infty}
			\resN{\operatorname{wh}_{B, P_p}^i \l(1\r)} \\
	=& 0 + \sum_{i = 1}^{\infty} (1-p) \cdot p^{i-1} X^{i-1} F^1 \\
	 & \explain{factor out, transform indices} \\
	=& (1-p) \cdot \sum_{i = 0}^{\infty} p^i X^i F^1 \\
	 & \explain{closed form of geometric series} \\
	=& \frac{(1-p) F}{1 - p X}
\end{align*}